@prefix rdf: <http://www.w3.org/1999/02/22-rdf-syntax-ns#> .
@prefix dc: <http://purl.org/dc/elements/1.1/> .
@prefix dcterms: <http://purl.org/dc/terms/> .
@prefix foaf: <http://xmlns.com/foaf/0.1/> .
@prefix rdfs: <http://www.w3.org/2000/01/rdf-schema#> .
@prefix xsd: <http://www.w3.org/2001/XMLSchema#> .
@prefix owl: <http://www.w3.org/2002/07/owl#> .

@prefix gov: <http://data.cabinetoffice.gov.uk/> .

# ====== DATA TYPES ======
gov:officialLabel a owl:DatatypeProperty ;
    rdfs:subPropertyOf rdfs:label ;
    rdfs:domain gov:Role , gov:Organisation ;
    rdfs:range xsd:string .

gov:unofficialLabel a owl:DatatypeProperty ;
    rdfs:subPropertyOf rdfs:label ;
    rdfs:domain gov:Role , gov:Organisation ;
    rdfs:range xsd:string .

gov:acronym a owl:DatatypeProperty ;
    rdfs:subPropertyOf rdfs:label ;
    rdfs:domain gov:Role , gov:Organisation ;
    rdfs:range xsd:string .

# ====== CLASSES ======

gov:Thing a owl:Class ;
    rdfs:label "Thing"@en ;
    rdfs:comment "Any idea, material thing, or event within the realm of human experience."@en .

# ====== ROLES ======
gov:Role rdfs:subClassOf gov:Thing ;
    rdfs:label "Role"@en ;
    rdfs:comment "A job or responsibility which can be inhabited by a Person."@en .

# === Political Roles, i.e. Ministers ===
gov:Minister rdfs:subClassOf gov:Role ;
    rdfs:label "Minister"@en ;
    rdfs:comment "A person (usually a member of Parliament) who is responsible for some government function."@en .

gov:PrimeMinister rdfs:subClassOf gov:Minister ;
    rdfs:label "Prime Minister"@en ;
    gov:officialLabel "First Lord of the Treasury"@en ;
    gov:acronym "PM" .

gov:SecretaryOfState rdfs:subClassOf gov:Minister ;
    rdfs:label "Secretary of State"@en ;
    gov:officialLabel "Secretary of State"@en ;
    rdfs:comment """His Majesty's principal secretaries of state, or secretaries of state, are senior
        ministers of the Crown in the Government of the United Kingdom. Secretaries of state
        head most major government departments and make up the majority of the Cabinet of the
        United Kingdom."""@en .

gov:MinisterOfState rdfs:subClassOf gov:Minister ;
    rdfs:label "Minister of State"@en ;
    gov:officialLabel "Minister of State"@en ;
    rdfs:comment """A Minister of State is a member of His Majesty's Government, junior only to
        a Secretary of State but senior to a Parliamentary Under-Secretary of State and
        Parliamentary Private Secretaries (PPSs). Ministers of State are responsible to
        their Secretaries of State."""@en .

gov:ParliamentaryUnderSecretary rdfs:subClassOf gov:Minister ;
    rdfs:label "Parliamentary under-secretary of State" ;
    gov:officialLabel "Parliamentary under-secretary of State"@en ;
    rdfs:comment  """The parliamentary under-secretary of state (or just parliamentary secretary, 
        particularly in departments not led by a Secretary of State) is the lowest of three
        tiers of government minister in the UK government, immediately junior to a Minister of State, 
        which is itself junior to a Secretary of State.
        """@en .

gov:ParliamentarySecretary rdfs:subClassOf gov:Minister ;
    gov:officialLabel "Parliamentary Secretary"@en ;
    rdfs:label "Parliamentary Secretary"@en ;
    rdfs:comment """Equivalent but not identical to a gov:ParliamentaryUnderSecretary"""@en .

gov:ParliamentaryPrivateSecretary rdfs:subClassOf gov:Role ;
    rdfs:label "Parliamentary Private Secretary"@en ;
    gov:officialLabel "Parliamentary Private Secretary"@en ;
    rdfs:comment """Not a government role, but they assist ministers in Parliament."""@en .

# === Administrative and Advisory Roles ===
gov:CivilServant rdfs:subClassOf gov:Role ;
    rdfs:label "Civil servant"@en ;
    gov:officialLabel "Civil servant"@en ;
    rdfs:comment """A servant of the Crown working in a civil capacity who is not the holder
        of a political (or judicial) office; the holder of certain other offices in respect of
        whose tenure of office special provision has been made; [or] a servant of the Crown in a
        personal capacity paid from the Civil List"""@en .

gov:SpecialAdvisor rdfs:subClassOf gov:Role ;
    rdfs:label "Special Advisor"@en ;
    gov:officialLabel "Special Advisor"@en ;
    gov:unofficialLabel "SpAd"@en ;
    rdfs:comment  """A special adviser, also known as a spad, is a temporary civil servant who advises 
        and assists UK government ministers[4] or ministers in the Scottish and Welsh devolved governments.
        They differ from impartial civil servants in that they are political appointees."""@en .

gov:PermanentSecretary rdfs:subClassOf gov:CivilServant ;
    rdfs:label "Permanent secretary" ;
    gov:officialLabel "Permanent under-secretary of state"@en ;
    gov:unofficialLabel "Perm Sec"@en ;
    rdfs:comment """The most senior civil servant of a ministry,
        charged with running the department on a day-to-day basis."""@en .

gov:CabinetSecretary rdfs:subClassOf gov:PermanentSecretary ;
    rdfs:label "Cabinet secretary"@en ;
    gov:officialLabel "Cabinet secretary"@en ;
    gov:unofficialLabel "Cab Sec"@en ;
    rdfs:comment "The most senior civil servant who acts as the senior policy advisor to the Prime Minister."@en .

gov:SecondPermanentSecretary rdfs:subClassOf gov:CivilServant .

gov:DirectorGeneral rdfs:subClassOf gov:CivilServant .

gov:Director rdfs:subClassOf gov:CivilServant .

gov:DeputyDirector rdfs:subClassOf gov:CivilServant .

# === Organisations ===
gov:Organisation rdfs:subClassOf gov:Thing .

gov:PublicBody rdfs:subClassOf gov:Organisation .

# List "maintained by the Cabinet Office" apparently: https://www.gov.uk/government/organisations

# Executive office - ex: Prime Minister's Office, 10 Downing Street
gov:Department rdfs:subClassOf gov:Organisation .
gov:ExecutiveOffice rdfs:subClassOf gov:Department .
# Ministerial department - ex: Department for Education
gov:MinisterialDepartment rdfs:subClassOf gov:Department .
# Non-ministerial department - ex: Competition and Markets Authority
gov:NonMinisterialDepartment rdfs:subClassOf gov:Department .

gov:ArmsLengthBody rdfs:subClassOf gov:PublicBody .
# Executive agency - ex: Companies House
gov:ExecutiveAgency rdfs:subClassOf gov:ArmsLengthBody .
gov:NonDepartmentalPublicBody rdfs:subClassOf gov:ArmsLengthBody .
# Executive non-departmental public body - ex: UKRI
gov:ExecutiveNonDepartmentalPublicBody rdfs:subClassOf gov:NonDepartmentalPublicBody .
# Advisory non-departmental public body - ex: Committee on Standards in Public Life
gov:AdvisoryNonDepartmentalPublicBody rdfs:subClassOf gov:NonDepartmentalPublicBody .
# Ad-hoc advisory group - ex: The Queen Elizabeth Memorial Committee
# Tribunal - ex: Competition Appeal Tribunal
# Public corporation - ex: BBC, Royal Parks
gov:PublicCorporation rdfs:subClassOf gov:PublicBody .
# Special health authority - ex: NHS Blood and Transplant
# Devolved administrations - ex: Welsh Government

# NB: this list doesn't include "SIS", "GCHQ", "Crown Estate", "Royal Mint"